progs/verif1.v
@@ -6,7 +6,234 @@ Import SequentialClight.SeqC.CSL.
 Require Import progs.client_lemmas.
 Require Import progs.list.
 
-Instance Cassert: ClassicalSep assert := _.
+
+Instance Nassert: NatDed assert := _.
+Instance Sassert: SepLog assert := _.
+Instance Cassert: ClassicalSep assert := _. 
+Instance Iassert: Indir assert := _.
+Instance SIassert: SepIndir assert := _.
+
+Local Open Scope logic.
+
+Lemma local_unfold: forall P rho, local P rho = !! (P rho).
+Proof. reflexivity. Qed.
+Hint Rewrite local_unfold : normalize.
+Lemma lift2_unfold: forall {A1 A2 B} (f: A1 -> A2 -> B) a1 a2 rho,
+        lift2 f a1 a2 rho = f (a1 rho) (a2 rho).
+Proof. reflexivity. Qed.
+Lemma lift1_unfold: forall {A1 B} (f: A1 -> B) a1 rho,
+        lift1 f a1 rho = f (a1 rho).
+Proof. reflexivity. Qed.
+Hint Rewrite @lift2_unfold @lift1_unfold : normalize.
+
+
+Lemma andp_unfold: forall P Q rho,
+  @andp assert Nassert P Q rho = @andp mpred Nveric (P rho) (Q rho).
+Proof. reflexivity. Qed.
+Hint Rewrite andp_unfold: normalize.
+
+Lemma prop_and {A} {NA: NatDed A}: 
+    forall P Q: Prop, prop (P /\ Q) = (prop P && prop Q).
+Proof. intros. apply pred_ext. apply prop_left. intros [? ?]; normalize.
+   normalize. apply prop_left; normalize.
+Qed.
+Hint Rewrite @prop_and : normalize.
+
+Lemma exp_unfold : forall A P rho,
+ @exp assert Nassert A P rho = @exp mpred Nveric A (fun x => P x rho).
+Proof.
+intros. reflexivity. 
+Qed.
+Hint Rewrite exp_unfold: normalize.
+
+Definition PROPx (P: list Prop) (Q: assert) := andp (prop (fold_right and True P)) Q.
+
+Notation "'PROP' ( x ; .. ; y )   z" := (PROPx (cons x%type .. (cons y%type nil) ..) z) (at level 10) : logic.
+Notation "'PROP' ()   z" :=   (PROPx nil z) (at level 10) : logic.
+Notation "'PROP' ( )   z" :=   (PROPx nil z) (at level 10) : logic.
+
+Definition LOCALx (Q: list (environ -> Prop)) (R: assert) := 
+                 andp (local (fold_right (lift2 and) (lift0 True) Q)) R.
+
+Notation " 'LOCAL' ( )   z" := (LOCALx nil z)  (at level 9) : logic.
+Notation " 'LOCAL' ()   z" := (LOCALx nil z)  (at level 9) : logic.
+
+Notation " 'LOCAL' ( x ; .. ; y )   z" := (LOCALx (cons x%type .. (cons y%type nil) ..) z)
+         (at level 9) : logic.
+
+Definition SEPx (R: list assert) : assert := fold_right sepcon emp R.
+
+Notation " 'SEP' ( x * .. * y )" := (SEPx (cons x%logic .. (cons y%logic nil) ..))
+         (at level 8) : logic.
+
+Notation " 'SEP' ( ) " := (SEPx nil) (at level 8) : logic.
+Notation " 'SEP' () " := (SEPx nil) (at level 8) : logic.
+
+Definition do_canon := (@sepcon assert _ _).
+
+Lemma canon1: forall P1 B  P Q R,
+   do_canon (prop P1 && B) (PROPx P (LOCALx Q (SEPx R))) = do_canon B  (PROPx (P1::P) (LOCALx Q (SEPx R))).
+Proof.
+unfold do_canon, PROPx, LOCALx, SEPx; intros.
+extensionality rho.
+simpl.
+normalize.
+rewrite andp_assoc.
+f_equal.
+Qed.
+
+Lemma canon2: forall Q1 B P Q R,
+    do_canon (local Q1 && B) (PROPx P (LOCALx Q (SEPx R))) = do_canon B (PROPx (P) (LOCALx (Q1::Q) (SEPx R))).
+Proof.
+unfold do_canon, PROPx, LOCALx, SEPx; intros.
+extensionality rho.
+simpl.
+normalize.
+rewrite andp_assoc.
+f_equal.
+Qed.
+
+Definition nonlocal (Q: assert) := True.
+
+Ltac check_nonlocal :=
+  match goal with
+  |  |- nonlocal (local _) => fail 1 
+  |  |- nonlocal (prop _) => fail 1 
+  |  |- nonlocal (andp _ _) => fail 1
+  |  |- nonlocal (sepcon _ _) => fail 1
+  | |- _ => apply I
+ end.
+
+Lemma canon3: forall R1 B P Q R,
+    nonlocal R1 ->
+    do_canon (B * R1) (PROPx P (LOCALx Q (SEPx R))) = do_canon B (PROPx (P) (LOCALx Q (SEPx (R1::R)))).
+Proof.
+unfold do_canon, PROPx, LOCALx, SEPx; intros.
+clear H.
+extensionality rho.
+simpl.
+rewrite sepcon_assoc.
+f_equal.
+rewrite sepcon_andp_prop.
+f_equal.
+normalize.
+Qed.
+
+Lemma canon4: forall P, do_canon emp P = P. 
+Proof.
+apply emp_sepcon.
+Qed.
+
+Lemma canon7: forall R1 P Q R, 
+   nonlocal R1 -> 
+   do_canon R1 (PROPx P (LOCALx Q (SEPx R))) = (PROPx P (LOCALx Q (SEPx (R1::R)))).
+Proof.
+unfold do_canon, PROPx, LOCALx, SEPx; intros.
+extensionality rho.
+simpl.
+normalize.
+Qed.
+ 
+Lemma canon8: forall R1 R2 R3 PQR,
+    do_canon ((R1 && R2) && R3) PQR = do_canon (R1 && (R2 && R3)) PQR.
+Proof. intros; rewrite andp_assoc; auto. 
+Qed.
+
+Lemma start_canon: forall P, P  = do_canon P (PROPx nil (LOCALx nil (SEPx nil ))).
+Proof.
+unfold do_canon, PROPx, LOCALx, SEPx; intros.
+extensionality rho; simpl.
+normalize.
+Qed.
+
+Hint Rewrite canon1 canon2 canon4 canon8 : canon.
+Hint Rewrite canon3 using check_nonlocal : canon.
+Hint Rewrite canon7 using check_nonlocal : canon.
+Hint Rewrite <- (@sepcon_assoc assert _) : canon.
+
+
+Definition islocal (P: assert) := exists Q, P = local Q.
+Lemma islocal_local: forall Q, islocal (local Q).
+Proof. intros; econstructor; eauto. Qed.
+
+Lemma islocal_andp: forall P Q, islocal P -> islocal Q -> islocal (P && Q).
+Proof.
+ intros. destruct H; destruct H0; subst.
+  exists (fun rho, x rho /\ x0 rho).
+ extensionality rho.
+ unfold local, lift1. simpl.
+ apply pred_ext; normalize.
+Qed.
+
+Lemma islocal_prop: forall Q, islocal (prop Q).
+Proof.
+intros. exists (fun rho => Q). unfold local, lift1. extensionality rho; simpl. auto.
+Qed.
+Hint Resolve islocal_local islocal_andp islocal_prop: local canon.
+
+Lemma canon5: forall Q R S, 
+       nonlocal Q ->
+       Q && (local R && S) = local R && (Q && S).
+Admitted.
+
+
+Lemma canon5b: forall Q R S, 
+       nonlocal Q ->
+       Q && (S && local R) = local R && (Q && S).
+Admitted.
+
+Lemma canon5c: forall Q R, 
+       nonlocal Q ->
+       (Q && local R) = local R && Q.
+Admitted.
+
+Lemma canon6: forall Q R S, 
+       nonlocal Q ->
+       Q && (prop R && S) = prop R && (Q && S).
+Admitted.
+
+Lemma canon6b: forall Q R S, 
+       nonlocal Q ->
+       Q && (S && prop R) = prop R && (Q && S).
+Admitted.
+
+Lemma canon6c: forall Q R, 
+       nonlocal Q ->
+       (Q && prop R) = prop R && Q.
+Admitted.
+
+Hint Rewrite canon5 using check_nonlocal : canon.
+Hint Rewrite canon5b using check_nonlocal : canon.
+Hint Rewrite canon5c using check_nonlocal : canon.
+Hint Rewrite canon6 using check_nonlocal : canon.
+Hint Rewrite canon6b using check_nonlocal : canon.
+Hint Rewrite canon6c using check_nonlocal : canon.
+
+Lemma finish_canon: forall R1 P Q R, 
+   do_canon R1 (PROPx P (LOCALx Q (SEPx R))) = (PROPx P (LOCALx Q (SEPx (R1::R)))).
+Proof.
+unfold do_canon, PROPx, LOCALx, SEPx; intros.
+extensionality rho.
+simpl.
+normalize.
+Qed.
+
+Goal forall (foo: environ -> Prop)(P: Prop) (Q: assert), 
+   Q && (local foo && prop P) =  (PROP(P) LOCAL (foo) SEP (Q)).
+intros.
+ etransitivity.
+ rewrite (start_canon (Q && (local foo && prop P))).
+ autorewrite with canon. reflexivity.
+ auto.
+Qed.
+
+Ltac canonicalize_pre :=
+  match goal with |- semax _ _ ?P _ _ =>
+      rewrite (start_canon P); autorewrite with canon
+  end.    
+
+Check (PROP(True) LOCAL (lift0 False) SEP (emp * emp)%logic)%logic.
+Check (PROP (True) SEP (emp))%logic.
 
 Require progs.test1.
 Module P := progs.test1.
@@ -27,42 +254,6 @@ Defined.
 Definition int2valt (i: int) := (Vint i, P.t_int).
 
 Definition ilseg (s: list int) p q := lseg P.t_listptr (map Vint s) p q.
-
-(*
-Definition ilseg (s: list int) (p q: expr) : assert
-   := fun rho => lseg P.t_listptr (map Vint s) (eval_expr rho p) (eval_expr rho q).
-*)
-
-Definition sumlist_spec :=
- DECLARE P.i_sumlist
-  WITH contents 
-  PRE [ p : P.t_listptr]  ilseg contents p nullval
-  POST [ i : P.t_int ] prop (i = Vint (fold_right Int.add Int.zero contents)).
-
-Definition reverse_spec :=
- DECLARE P.i_reverse
-  WITH contents : list int
-  PRE  [ p : P.t_listptr ] ilseg contents p nullval
-  POST [p : P.t_listptr ] ilseg (rev contents) p nullval.
-
-Definition main_spec := (P.i_main, mk_funspec (Tnil, P.t_int) _ (main_pre P.prog) (main_post P.prog)).
-
-Definition Gprog : funspecs := 
-   sumlist_spec :: reverse_spec :: main_spec::nil.
-
-Definition sumlist_Inv (contents: list int) : assert :=
-          (EX cts: list int, 
-           (fun rho => !!(fold_right Int.add Int.zero contents =
-             Int.add (force_int (eval_expr (Etempvar P.i_s P.t_int) rho))
-                       (fold_right Int.add Int.zero cts))) &&
-           (fun rho => ilseg cts (eval_expr (Etempvar P.i_t P.t_listptr) rho) nullval)).
-
-Definition sumlist_Inv' (contents: list int) (rho: environ) : mpred :=
-          (EX cts: list int, 
-           !!(fold_right Int.add Int.zero contents =
-             Int.add (force_int (eval_expr (Etempvar P.i_s P.t_int) rho))
-                       (fold_right Int.add Int.zero cts)) &&
-           ilseg cts (eval_expr (Etempvar P.i_t P.t_listptr) rho) nullval).
 
 Definition semax_body' (G:  funspecs) (f: function) (spec: ident * funspec) :=
   match spec with (i, mk_funspec _ A pre post) => semax_body G f A pre post end.
@@ -108,9 +299,9 @@ Hint Rewrite Int.add_zero  Int.add_zero_l Int.sub_zero_l : normalize.
 Lemma lseg_unroll': forall T {ls: listspec T} l x z , 
     lseg T l x z = (!! (ptr_eq x z) && !! (l=nil) && emp) || 
                           (EX h:val, EX r:list val, EX y:val, 
-                          !! (~ptr_eq x z) &&  !!(l=h::r) && 
-                       field_mapsto Share.top list_data (x, list_struct) (h, list_dtype) 
-                      * field_mapsto Share.top list_link (x, list_struct) (y, T)
+                          !! (ptr_neq x z) &&  !!(l=h::r) && 
+                       field_mapsto Share.top list_struct list_data x h 
+                      * field_mapsto Share.top list_struct list_link x y
                       * |> lseg T r y z).
 Proof.
 intros.
@@ -138,12 +329,12 @@ apply exp_right with x2.
 normalize.
 Qed.
 
-Definition ilseg_nil (l: list  int) x z := !! (ptr_eq x z) && !! (l=nil) && emp.
-Definition ilseg_cons l x z := 
+Definition ilseg_nil (l: list  int) x z : mpred := !! (ptr_eq x z) && !! (l=nil) && emp.
+Definition ilseg_cons l x z : mpred := 
                           (EX h:int, EX r:list int, EX y:val, 
-                          !! (~ptr_eq x z) &&  !!(l=h::r) && 
-                       field_mapsto Share.top list_data (x, list_struct) (Vint h, P.t_int) 
-                      * field_mapsto Share.top list_link (x, list_struct) (y, P.t_listptr)
+                          !! (ptr_neq x z) &&  !!(l=h::r) && 
+                       field_mapsto Share.top list_struct list_data x (Vint h) 
+                      * field_mapsto Share.top list_struct list_link x y
                       * |> ilseg r y z).
 
 Lemma ilseg_unroll': forall l x z , 
@@ -190,146 +381,533 @@ apply expr_true_Cnot_ptr; auto.
 Qed.
 Hint Rewrite expr_true_Cnot_ptr' using (solve [simpl; auto]) : normalize.
 
-Lemma local_unfold: forall P rho, local P rho = !! (P rho).
+Lemma fst_unfold: forall {A B} (x: A) (y: B), fst (x,y) = x.
 Proof. reflexivity. Qed.
-Hint Rewrite local_unfold : normalize.
+Lemma snd_unfold: forall {A B} (x: A) (y: B), snd (x,y) = y.
+Proof. reflexivity. Qed.
+Hint Rewrite @fst_unfold @snd_unfold : normalize.
+
+Lemma ilseg_eq: forall s p, 
+   typecheck_val p P.t_listptr = true -> 
+    (ilseg s p p = !!(s=nil) && emp).
+Proof. intros. unfold ilseg. rewrite lseg_eq; auto. f_equal. f_equal.
+ apply prop_ext. destruct s; simpl; intuition congruence.
+Qed.
+Hint Rewrite ilseg_eq : normalize.
+
+
+Definition strict_bool_val (v: val) (t: type) : option bool :=
+  match v, t with
+  | Vint n, Tint _ _ _ => Some (negb (Int.eq n Int.zero))
+  | Vint n, (Tpointer _ _ | Tarray _ _ _ | Tfunction _ _) =>
+            if Int.eq n Int.zero then Some false else None
+  | Vptr b ofs, (Tpointer _ _ | Tarray _ _ _ | Tfunction _ _) => Some true
+  | Vfloat f, Tfloat sz _ => Some (negb(Float.cmp Ceq f Float.zero))
+  | _, _ => None
+  end.
+
+Definition typed_true (t: type) (v: val)  : Prop := strict_bool_val v t = Some true.
+Definition typed_false (t: type)(v: val) : Prop := strict_bool_val v t = Some false.
+
+Lemma HACK_expr_true:  forall e,
+    expr_true e = lift1 (typed_true (typeof e)) (eval_expr e).
+Proof.
+(* NOT TRUE, but when we use strict_bool_val in the SeparationLogic then it will be true *)
+Admitted.
+
+
+Lemma ilseg_nonnull:
+  forall s v,
+      typed_true P.t_listptr v ->
+     ilseg s v nullval = ilseg_cons s v nullval.
+Proof.
+intros. subst. 
+rewrite ilseg_unroll'.
+unfold ilseg_cons, ilseg_nil.
+apply pred_ext; normalize.
+apply orp_left; auto. normalize.
+unfold typed_true, strict_bool_val,ptr_eq in *.
+destruct v; simpl in *; try contradiction.
+rewrite H0 in H. inv H.
+intros.
+apply orp_right2. apply exp_right with x; normalize. apply exp_right with x0; normalize.
+apply exp_right with x1; normalize.
+Qed.
+
+Lemma ilseg_nonnull':
+  forall e' rho s e,
+    expr_true e' rho ->
+    e = eval_expr e' rho ->
+     ilseg s e nullval = ilseg_cons s e nullval.
+Proof.
+intros. subst. 
+rewrite ilseg_unroll'.
+unfold ilseg_cons, ilseg_nil.
+apply pred_ext; normalize.
+apply orp_left; auto. normalize.
+unfold expr_true, bool_val,ptr_eq in *.
+destruct (eval_expr e' rho); simpl in *; try contradiction.
+rewrite H0 in H. destruct (typeof e'); inv H.
+intros.
+apply orp_right2. apply exp_right with x; normalize. apply exp_right with x0; normalize.
+apply exp_right with x1; normalize.
+Qed.
+
+Lemma lift2_ilseg_cons: 
+ forall s p q, lift2 (ilseg_cons s)  p q =
+    EX h:int, EX r: list int, EX y: val,
+      local (lift2 ptr_neq p q) &&
+      !! (s = h::r) &&
+      lift2 (field_mapsto Share.top list_struct list_data) p (lift0 (Vint h)) *
+      lift2 (field_mapsto Share.top list_struct list_link) p (lift0 y) *
+      |> lift2 (ilseg r) (lift0 y) q.
+Proof. reflexivity. Qed.
+Hint Rewrite lift2_ilseg_cons : normalize.
+
+Lemma local_andp_prop:  forall P Q, local P && prop Q = prop Q && local P.
+Proof. intros. apply andp_comm. Qed.
+Lemma local_andp_prop1: forall P Q R, local P && (prop Q && R) = prop Q && (local P && R).
+Proof. intros. rewrite andp_comm. rewrite andp_assoc. f_equal. apply andp_comm. Qed.
+Hint Rewrite local_andp_prop local_andp_prop1 : normalize.
+
+Lemma local_sepcon_assoc1:
+   forall P Q R, (local P && Q) * R = local P && (Q * R).
+Proof.
+intros.
+extensionality rho; unfold local, lift1; simpl.
+apply pred_ext; normalize.
+Qed.
+Lemma local_sepcon_assoc2:
+   forall P Q R, R * (local P && Q) = local P && (R * Q).
+Proof.
+intros.
+extensionality rho; unfold local, lift1; simpl.
+apply pred_ext; normalize.
+Qed.
+Hint Rewrite local_sepcon_assoc1 local_sepcon_assoc2 : normalize.
+
+Lemma reassoc_local:
+  forall P Q R, local P && (local Q && R) = (local P && local Q) && R.
+Proof. intros. symmetry ; apply andp_assoc. Qed.
+
+Ltac strip1_later P :=
+ match P with 
+ | |> ?L && |> ?R => constr:(L && R)
+ | ?L && |> ?R => let Z := strip1_later L in constr:(Z && R)
+ | |> ?L && ?R => let Z := strip1_later R in constr:(L && Z)
+ | ?L && ?R => let L' := strip1_later L in let R' := strip1_later R in constr:(L' && R')
+ | |> ?L * |> ?R => constr:(L * R)
+ | ?L * |> ?R => let Z := strip1_later L in constr:(Z * R)
+ | |> ?L * ?R => let Z := strip1_later R in constr:(L * Z)
+ | ?L * ?R => let L' := strip1_later L in let R' := strip1_later R in constr:(L'*R')
+ | |> ?L => constr:(L)
+ | ?L => constr:(L)
+end.
+
+Lemma andp_later_derives {A} {NA: NatDed A}{IA: Indir A}:
+  forall P Q P' Q': A, P |-- |> P' -> Q |-- |> Q' -> P && Q |-- |> (P' && Q').
+Proof.
+intros. rewrite later_andp. apply andp_derives; auto. Qed.
+
+Lemma sepcon_later_derives {A} {NA: NatDed A}{SL: SepLog A}{IA: Indir A}{SI: SepIndir A}:
+  forall P Q P' Q': A, P |-- |> P' -> Q |-- |> Q' -> P * Q |-- |> (P' * Q').
+Proof.
+intros. rewrite later_sepcon. apply sepcon_derives; auto. Qed.
+
+Hint Resolve andp_later_derives sepcon_later_derives sepcon_derives
+              andp_derives imp_derives now_later derives_refl: derives.
+
+
+
+Lemma load_field_assoc:
+  forall P Q R S : assert, islocal Q ->
+            (P && |> (Q && (R * S))) = (P && (|> (S * (Q && R)))).
+Proof.
+intros.
+f_equal.
+f_equal.
+destruct H as [Q' ?].
+subst.
+extensionality rho; unfold local, lift1; simpl.
+normalize.
+f_equal.
+apply sepcon_comm.
+Qed.
+
+Lemma cconv_sepcon1 {A}{ND: NatDed A}{SA: SepLog A}:
+  forall P Q Q': A,  Q |-- Q' -> P * Q |-- P * Q'.
+Proof. 
+ intros. apply sepcon_derives; auto.
+Qed.
+Lemma cconv_sepcon2 {A}{ND: NatDed A}{SA: SepLog A}:
+  forall P Q Q': A,  Q |-- Q' -> Q * P |-- Q' * P.
+Proof. 
+ intros. apply sepcon_derives; auto.
+Qed.
+Lemma cconv_andp1 {A}{ND: NatDed A}:
+  forall P Q Q': A,  Q |-- Q' -> P && Q |-- P && Q'.
+Proof. 
+ intros. apply andp_derives; auto.
+Qed.
+Lemma cconv_andp2 {A}{ND: NatDed A}:
+  forall P Q Q': A,  Q |-- Q' -> Q && P |-- Q'  && P.
+Proof. 
+ intros. apply andp_derives; auto.
+Qed.
+
+Hint Resolve @cconv_sepcon1 @cconv_sepcon2 @cconv_andp1 @cconv_andp2 : cconv.
+
+Definition sumlist_spec :=
+ DECLARE P.i_sumlist
+  WITH contents 
+  PRE [ p : P.t_listptr]  ilseg contents p nullval
+  POST [ i : P.t_int ]  prop (i = Vint (fold_right Int.add Int.zero contents)).
+
+Definition reverse_spec :=
+ DECLARE P.i_reverse
+  WITH contents : list int
+  PRE  [ p : P.t_listptr ] ilseg contents p nullval
+  POST [p : P.t_listptr ] ilseg (rev contents) p nullval.
+
+Definition main_spec := (P.i_main, mk_funspec (Tnil, P.t_int) _ (main_pre P.prog) (main_post P.prog)).
+
+Definition Gprog : funspecs := 
+   sumlist_spec :: reverse_spec :: main_spec::nil.
+
+Definition partial_sum (contents cts: list int) (v: val) := 
+     fold_right Int.add Int.zero contents = Int.add (force_int  v) (fold_right Int.add Int.zero cts).
+
+Definition sumlist_Inv (contents: list int) : assert :=
+          (EX cts: list int, 
+            PROP () LOCAL (lift1 (partial_sum contents cts) (eval_id P.i_s)) 
+            SEP (lift2 (ilseg cts) (eval_id P.i_t) (lift0 nullval))).
+
+Lemma closed_wrt_local_and: forall S P Q,
+  closed_wrt_vars S (local P) ->
+  closed_wrt_vars S (local Q) ->
+  closed_wrt_vars S (local (lift2 and P Q)).
+Proof.
+Admitted.
+Hint Resolve closed_wrt_local_and: closed.
+
+Lemma closed_wrt_local1: forall a b f, 
+  a <> b -> closed_wrt_vars (modified1 a) (local (lift1 f (eval_id b))).
+Proof.
+intros.
+intros rho ? ?.
+unfold local, lift1. f_equal.
+f_equal.
+unfold eval_id, force_val.
+simpl.
+destruct (H0 b). hnf in H1. subst; contradiction H; auto.
+rewrite H1; auto.
+Qed.
+Hint Extern 2 (closed_wrt_vars (modified1 _) (local (lift1 _ (eval_id _)))) => 
+      (apply closed_wrt_local1; solve [let Hx := fresh in (intro Hx; inv Hx)]) : closed.
+
+
+Lemma closed_wrt_local2: forall a b c f, 
+  a <> b -> a <> c -> closed_wrt_vars (modified1 a) (local (lift2 f (eval_id b) (eval_id c))).
+Proof.
+intros.
+intros rho ? ?.
+unfold local, lift1, lift2. f_equal.
+f_equal.
+admit.
+admit.
+Qed.
+Hint Extern 2 (closed_wrt_vars (modified1 _) (local (lift2 _ (eval_id _) (eval_id _)))) => 
+      (apply closed_wrt_local2; solve [let Hx := fresh in (intro Hx; inv Hx)]) : closed.
+
+Lemma closed_wrt_lift1: forall a b f, 
+  a <> b -> closed_wrt_vars (modified1 a) (lift1 f (eval_id b)).
+Proof.
+intros.
+intros rho ? ?.
+unfold lift1. f_equal.
+unfold eval_id, force_val.
+simpl.
+destruct (H0 b). hnf in H1. subst; contradiction H; auto.
+rewrite H1; auto.
+Qed.
+
+Hint Extern 2 (closed_wrt_vars (modified1 _) (lift1 _ (eval_id _))) => 
+      (apply closed_wrt_lift1; solve [let Hx := fresh in (intro Hx; inv Hx)]) : closed.
+
+Lemma closed_wrt_lift2: forall a b c f, 
+  a <> b -> a <> c -> closed_wrt_vars (modified1 a) (lift2 f (eval_id b) (eval_id c)).
+Proof.
+intros.
+intros rho ? ?.
+unfold lift2, lift1. f_equal.
+unfold eval_id, force_val.
+simpl.
+destruct (H1 b). hnf in H2. subst; contradiction H; auto.
+rewrite H2; auto.
+unfold eval_id, force_val.
+simpl.
+destruct (H1 c). hnf in H2. subst; contradiction H0; auto.
+rewrite H2; auto.
+Qed.
+Hint Extern 2 (closed_wrt_vars (modified1 _) (lift2 _ (eval_id _) (eval_id _))) => 
+      (apply closed_wrt_lift2; solve [let Hx := fresh in (intro Hx; inv Hx)]) : closed.
+(*
+Lemma closed_wrt_PROPx:
+ forall S P Q, closed_wrt_vars S Q -> closed_wrt_vars S (PROPx P Q).
+Proof.
+Admitted. 
+Hint Resolve closed_wrt_PROPx: closed.
+
+Lemma closed_wrt_LOCALx:
+ forall S Q R, closed_wrt_vars S (local Q) -> closed_wrt_vars S R -> closed_wrt_vars S (LOCALx Q R).
+Admitted. 
+Hint Resolve closed_wrt_LOCALx: closed.
+
+Lemma closed_wrt_SEPx: forall S P, closed_wrt_vars S P -> closed_wrt_vars S (SEPx P).
+Admitted. 
+Hint Resolve closed_wrt_SEPx: closed.
+Lemma closed_wrt_local_lift0: forall S Q, closed_wrt_vars S (local (lift0 Q)).
+Proof.
+intros. intro; intros. unfold local, lift1, lift0. auto.
+Qed.
+Hint Resolve closed_wrt_local_lift0: closed.
+
+*)
+
+Lemma forward_set:
+  forall Delta G P1 P2 P3 id e c Q,
+  typecheck_temp_id id (typeof e) Delta = true ->
+  temp_free_in id e = false ->
+  closed_wrt_vars (modified1 id) (PROPx P1 (LOCALx P2 (SEPx P3))) ->
+  (forall rho, tc_expr Delta e rho) ->
+  semax (set_temp_assigned Delta id) G
+             (PROPx P1 (LOCALx (lift2 eq (eval_id id) (eval_expr e) :: P2) (SEPx P3)))
+             c Q ->
+  semax Delta G (PROPx P1 (LOCALx P2 (SEPx P3))) (Ssequence (Sset id e) c) Q.
+Proof.
+intros.
+eapply forward_set; try eassumption.
+eapply semax_pre; try apply H3.
+unfold PROPx, LOCALx, SEPx; intro rho; simpl; normalize.
+Qed.
+
+
+Lemma insert_local: forall Q1 P Q R,
+  local Q1 && (PROPx P (LOCALx Q (SEPx R))) = (PROPx P (LOCALx (Q1 :: Q) (SEPx R))).
+Proof.
+intros. extensionality rho.
+unfold PROPx, LOCALx, SEPx, lift2.
+normalize.
+unfold local, lift1. simpl.
+f_equal.
+apply pred_ext; normalize.
+Qed.
+
+Lemma semax_pre:
+ forall P' Delta G P1 P2 P3 c R,
+     (PROPx P1 (LOCALx (tc_environ Delta :: P2) (SEPx P3))) |-- P' ->
+     semax Delta G P' c R  -> 
+     semax Delta G (PROPx P1 (LOCALx P2 (SEPx P3))) c R.
+Proof.
+intros.
+eapply semax_pre; try apply H0.
+ rewrite insert_local. auto.
+Qed.
+
+Ltac forward_while Inv Postcond :=
+  apply semax_pre with Inv; 
+  [ | apply semax_seq with Postcond;
+    [ apply semax_while ; [ | compute; auto | | ] | ]].
+
+Hint Rewrite insert_local:  normalize.
+
+Lemma exp_derives {A}{NA: NatDed A}{B}:
+   forall F G: B -> A, (forall x, F x |-- G x) -> exp F |-- exp G.
+Proof.
+intros.
+apply exp_left; intro x. apply exp_right with x; auto.
+Qed.
+
+Lemma lift_ilseg_cons_unfold:
+   forall s p q, lift2 (ilseg_cons s) p q =
+       EX h: int, EX r: list int, EX y: val,
+         local (lift2 ptr_neq p q) && !!(s = h :: r) &&
+         lift2 (field_mapsto Share.top list_struct list_data) p (lift0 (Vint h)) *
+         lift2 (field_mapsto Share.top list_struct list_link) p (lift0 y) * |> lift2 (ilseg r) (lift0 y) q.
+Proof. intros; extensionality rho; reflexivity.
+Qed.
+ 
+
+Ltac find_in_list A L :=
+ match L with 
+  | A :: _ => constr:(O)
+  | _ :: ?Y => let n := find_in_list A Y in constr:(S n)
+  | nil => fail
+  end.
+
+Fixpoint delete_nth {A} (n: nat) (xs: list A) {struct n} : list A :=
+ match n, xs with
+ | O, y::ys => ys
+ | S n', y::ys =>y :: delete_nth n' ys
+ | _ , _ => nil
+ end.
+
+
+Lemma grab_nth_LOCAL:
+   forall n B P Q R,
+    do_canon B (PROPx P (LOCALx Q (SEPx R))) = 
+    do_canon (local (nth n Q (lift0 True)) && B) (PROPx P (LOCALx Q (SEPx R))).
+Proof.
+intros n B P Q R; revert n Q B.
+induction n; intros.
+destruct Q; simpl nth.
+f_equal.
+extensionality rho; unfold local, lift0,lift1. simpl. normalize.
+rewrite canon2.
+f_equal.
+f_equal.
+extensionality rho; unfold LOCALx; simpl.
+f_equal.
+unfold local, lift1, lift2.
+f_equal.
+apply prop_ext; intuition.
+destruct Q; simpl nth.
+f_equal.
+extensionality rho; unfold local, lift0,lift1. simpl. normalize.
+rewrite <- canon2.
+rewrite <- canon2.
+rewrite IHn.
+f_equal.
+unfold local, lift0, lift1, lift2; extensionality rho.
+simpl.
+apply pred_ext; normalize.
+Qed.
+
+Lemma grab_nth_SEP:
+   forall n B P Q R,
+    do_canon B (PROPx P (LOCALx Q (SEPx R))) = do_canon (B* nth n R emp) (PROPx P (LOCALx Q (SEPx (delete_nth n R)))).
+Proof.
+intros n B P Q R; revert n R B.
+induction n; intros.
+destruct R.
+simpl nth.  unfold delete_nth.
+f_equal. extensionality rho; simpl; symmetry; apply sepcon_emp.
+simpl nth.
+unfold delete_nth.
+rewrite canon3 by apply I. auto.
+destruct R.
+simpl nth.  unfold delete_nth.
+f_equal. extensionality rho; simpl; symmetry; apply sepcon_emp.
+rewrite <- canon3 by apply I.
+rewrite (IHn _ (B*a)).
+simpl nth.
+replace (delete_nth (S n) (a::R)) with (a :: delete_nth n R) by reflexivity.
+rewrite <- canon3 by apply I.
+f_equal.
+repeat rewrite sepcon_assoc.
+f_equal.
+apply sepcon_comm.
+Qed.
+
+Lemma restart_canon: forall P Q R, (PROPx P (LOCALx Q (SEPx R))) = do_canon emp (PROPx P (LOCALx Q (SEPx R))).
+Proof.
+intros.
+unfold do_canon. rewrite emp_sepcon. auto.
+Qed.
+
+Lemma ilseg_nonnullx: 
+  forall s p q,
+   local (lift1 (typed_true P.t_listptr) p) && lift2 (ilseg s) p q = 
+   EX  h : int,
+      EX  r : list int,
+       EX  y : val,
+         local (lift2 ptr_neq p q) && !!(s = h :: r) &&
+         lift2 (field_mapsto Share.top list_struct list_data) p
+           (lift0 (Vint h)) *
+         lift2 (field_mapsto Share.top list_struct list_link) p (lift0 y) *
+         |>lift2 (ilseg r) (lift0 y) q.
+Admitted.
+
+Lemma exp_do_canon:
+   forall T (P: T -> assert) (Q: assert), do_canon (exp P) Q = EX x:_, do_canon (P x) Q.
+Proof. apply exp_sepcon1. Qed.
+Hint Rewrite exp_do_canon: canon.
+Hint Rewrite exp_do_canon: normalize.
+
+Ltac go_lower := 
+ let rho := fresh "rho" in intro rho; unfold PROPx, LOCALx, SEPx; simpl; normalize.
+
+Ltac change_in_pre S S' :=
+ match goal with |- semax _ _ ?P _ _ =>
+  match P with context C[S] =>
+     let P' := context C[S'] in apply semax_pre with P'; [go_lower | ]
+  end
+ end.
+
+Lemma semax_extract_PROP:
+  forall Delta G (PP: Prop) P QR c Post,
+       (PP -> semax Delta G (PROPx P QR) c Post) -> 
+       semax Delta G (PROPx (PP::P) QR) c Post.
+Proof.
+intros.
+apply client_lemmas.semax_pre with (!!PP && PROPx P QR).
+unfold PROPx in *; simpl. normalize.
+apply semax_extract_prop.
+auto.
+Qed.
 
 Lemma body_sumlist: semax_body' Gprog P.f_sumlist sumlist_spec.
 Proof.
 intro contents.
 simpl fn_body; simpl fn_params; simpl fn_return.
 normalize.
+change ( lift1 (fun p : val => ilseg contents p nullval) (eval_id P.i_p))
+  with (lift2 (ilseg contents) (eval_id P.i_p) (lift0 nullval)).
+
+canonicalize_pre.
+apply forward_set; [compute; auto | compute; auto | auto 50 with closed | compute; auto | ].
+admit. (* closed *)
 apply forward_set; [compute; auto | compute; auto | auto with closed | compute; auto | ].
-simpl @snd; simpl @fst.
-apply closed_wrt_andp.
-xxx...
-Search closed_wrt_vars.
-apply forward_set; [compute; auto | compute; auto | auto with closed | compute; auto | ].
+admit. (* closed *)
+
 forward_while (sumlist_Inv contents)
-    (fun rho => !!(fold_right Int.add Int.zero contents = force_int (eval_id P.i_s rho))).
+    (PROP() LOCAL (lift1 (fun v => fold_right Int.add Int.zero contents = force_int v) (eval_id P.i_s))SEP(TT)).
 (* Prove that current precondition implies loop invariant *)
-unfold sumlist_Inv; intros; simpl; normalize.
+unfold sumlist_Inv.
 apply exp_right with contents.
-rewrite H0. rewrite H1.  simpl.
+go_lower.
+rewrite H0. rewrite H1. simpl. unfold partial_sum.
 rewrite Int.add_zero_l. normalize.
 (* Prove that loop invariant implies typechecking condition *)
 intros; unfold tc_expr; simpl; normalize.
 (* Prove that invariant && not loop-cond implies postcondition *)
-intro rho.
-normalize.
 unfold sumlist_Inv.
-simpl.
-apply exp_left; intro cts.
-normalize.
-rewrite H0.
-rewrite H.
-unfold ilseg; rewrite lseg_eq; auto.
-normalize.
-destruct cts; inv H1. simpl. normalize.
+go_lower.
+intros cts ?.
+unfold partial_sum in H0;  rewrite H0. rewrite H. normalize.
 (* Prove that loop body preserves invariant *)
-unfold sumlist_Inv at 1. normalize.
-apply extract_exists_pre; auto;  intro cts.
-
-apply semax_pre with
-(local (expr_true (Etempvar P.i_t P.t_listptr)) &&
- (fun rho => !!(fold_right Int.add Int.zero contents =
-       Int.add (force_int (eval_id P.i_s rho))
-         (fold_right Int.add Int.zero cts))) &&
- (fun rho => ilseg_cons cts (eval_id P.i_t rho) nullval)).
-intro.
-simpl.
-rewrite ilseg_unroll'. auto.
-unfold ilseg_cons, ilseg_nil.
-intro.
+unfold sumlist_Inv at 1.
 normalize.
-apply orp_left.
+apply extract_exists_pre; intro cts.
+rewrite HACK_expr_true. simpl typeof.
 normalize.
-unfold expr_true, bool_val in H1. simpl in H1.
-unfold ptr_eq in H2. destruct (eval_id P.i_t rho); simpl in *; try contradiction.
-rewrite H2 in H1; inv H1.
-normalize. intros h r ? y.
-apply exp_right with h; normalize. apply exp_right with r; normalize.
-apply exp_right with y; normalize.
-unfold ilseg_cons.
-match goal with |- semax _ _ (_ && _ && ?P) _ _ => 
-  change P with (EX  h : int, EX  r : list int, EX  y : val,  
-      fun rho => !!(~ ptr_eq (eval_id P.i_t rho) nullval) && !!(cts = h :: r) &&
-      field_mapsto Share.top (eval_id P.i_t rho, list_struct) list_data
-        (Vint h, P.t_int) *
-      field_mapsto Share.top (eval_id P.i_t rho, list_struct) list_link
-        (y, P.t_listptr) * |>ilseg r y nullval)
- end.
-normalize. apply extract_exists_pre; [apply Int.zero | intro h].
-normalize. apply extract_exists_pre; [apply nil | intro r].
-normalize. apply extract_exists_pre; [apply Vundef | intro y].
-simpl.
+change_in_pre (ilseg cts) (ilseg_cons cts).
+   rewrite ilseg_nonnull by auto.
+   unfold ilseg_cons.
+   normalize; intros h r ? y.
+   apply exp_right with h; normalize.
+   apply exp_right with r; normalize.
+   apply exp_right with y; normalize.
+rewrite lift_ilseg_cons_unfold.
+rewrite restart_canon; rewrite (grab_nth_SEP 0);
+   unfold nth, delete_nth.
+   normalize; apply extract_exists_pre; intro h.
+   normalize; apply extract_exists_pre; intro r.
+   normalize; apply extract_exists_pre; intro y.
+   autorewrite with canon.
+apply semax_extract_PROP; intro. subst.
 
-match goal with |- semax _ _ ?P _ _ => 
-  apply semax_pre with (!!(cts = h::r) && P)
-end.
-intro; normalize.
-apply semax_extract_prop.
-intro; subst cts.
-(*
-apply semax_pre with
-  (fun rho : environ =>
-  !!(map (fun i : int => (Vint i, P.t_int)) cts = (h, P.t_int) :: r /\
-      typecheck_val h P.t_int = true /\ typecheck_val y P.t_listptr = true) &&
-   (expr_true (Etempvar P.i_t P.t_listptr) rho &&
-   !!(fold_right Int.add Int.zero contents =
-      Int.add (force_int (eval_id rho P.i_s))
-        (fold_right Int.add Int.zero cts)) &&
-   field_mapsto Share.top (eval_id rho P.i_t, P.t_list) P.i_h  (h, P.t_int) *
-   field_mapsto Share.top (eval_id rho P.i_t, P.t_list) P.i_t  (y, P.t_listptr) *
-     |>lseg r (y, P.t_listptr) (nullval, P.t_listptr))).
-intros.
-unfold expr_true.
-normalize.
-apply semax_extract_prop.
-intros [? [? ?]].
-set (e1:= Ederef (Etempvar P.i_t P.t_listptr) P.t_list).
-set (P := (fun rho0 : environ =>
-         expr_true (Etempvar P.i_t P.t_listptr) rho0 &&
-         !!(fold_right Int.add Int.zero contents =
-            Int.add (force_int (eval_expr rho0 (Etempvar P.i_s P.t_int)))
-              (fold_right Int.add Int.zero cts)) &&
-         !!(map (fun i : int => (Vint i, P.t_int)) cts = (h, P.t_int) :: r /\
-            typecheck_val h P.t_int = true /\
-            typecheck_val y P.t_listptr = true) &&
-         field_mapsto Share.top
-           (eval_expr rho0 (Etempvar P.i_t P.t_listptr), P.t_list) P.i_t
-           (y, P.t_listptr) *
-         |>lseg r (y, P.t_listptr) (nullval, P.t_listptr))).
 
-apply semax_pre with
- (fun rho => |> (field_mapsto Share.top (eval_lvalue rho e1, P.t_list) P.i_h
-     (h, P.t_int) 
-   * subst P.i_h h P rho)).
-intros.
-
-admit.
-eapply sequential; [intros; simpl; reflexivity | ].
-pose (Q := 
-       ((fun rho => field_mapsto Share.top ((eval_lvalue rho e1), typeof e1) P.i_h (h, P.t_int)) * P)).
-apply semax_seq with Q.
-apply semax_post with (normal_ret_assert Q).
-normalize.
-evar (Q3: assert).
-apply semax_pre with Q3; [ unfold Q3 |  unfold Q3; eapply semax_load_field; eauto].
-intros. unfold e1.
-simpl.
-apply andp_right.
-apply prop_right.
-simpl. split3; auto. split; auto.
-clear - H2.
-admit.  (* typechecking proof *)
-auto.
-unfold e1.
-admit.  (* easy *) 
-simpl. reflexivity.
-simpl. reflexivity.
-simpl. rewrite if_true by auto. reflexivity.
-*)
 
 Admitted.
 
